wand1

theories/SLFWP.v
@@ -1,5 +1,130 @@
 
 
+
+-------
+
+
+Definition wpgen_fail : formula := fun Q =>
+  \[False].
+
+Definition wpgen_val (v:val) : formula := fun Q =>
+  Q v.
+
+Definition wpgen_let (F1:formula) (F2of:val->formula) : formula := fun Q =>
+  F1 (fun X => F2of X Q).
+
+Definition wpgen_seq (F1 F2:formula) : formula := fun Q =>
+  F1 (fun X => F2 Q).
+
+Definition wpgen_app (t1:trm) (t2:trm) : formula := fun Q =>  
+  wp (trm_app t1 t2) Q.
+
+Definition wpgen_if_val (v:val) (F1 F2:formula) : formula := fun Q =>
+  \exists (b:bool), \[v = val_bool b] \* (if b then F1 Q else F2 Q).
+
+Definition wpgen_if (F0 F1 F2:formula) : formula :=
+  wpgen_let F0 (fun v => wpgen_if_val v F1 F2).
+
+Fixpoint wpgen (t:trm) : formula :=
+  match t with
+  | trm_val v => wpgen_val v
+  | trm_var x => wpgen_fail
+  | trm_fun x t1 => wpgen_val (val_fun x t1)
+  | trm_fix f x t1 => wpgen_val (val_fix f x t1)
+  | trm_if t0 t1 t2 => wpgen_if (wpgen t0) (wpgen t1) (wpgen t2)
+  | trm_let x t1 t2 => wpgen_let (wpgen t1) (fun X => wpgen (subst x X t2))
+  | trm_app t1 t2 => wgpen_app t1 t2
+  end.
+
+
+Lemma wpgen_himpl_wp : forall t Q,
+  H ==> wpgen t Q ->
+  triple t H Q.
+
+  H ==> wp t Q ->
+  triple t H Q.
+
+  H ==> wpgen t Q ->
+  H ==> wp t Q ->
+
+  wpgen t Q ==> wp t Q.
+
+(in details)
+
+then derive
+
+  Lemma triple_of_wpgen : forall t Q,
+    H ==> wpgen t Q ->
+    triple t H Q.
+
+
+
+
+Lemma wpgen_himpl_wp : forall t Q,
+  wpgen t Q ==> wp t Q.
+
+Definition wpgen_sound_for t := forall Q,
+  wpgen t Q ==> wp t Q.
+
+wpgen_sound_for (trm_val v)
+wpgen_sound_for (trm_fun x t).
+wpgen_sound_for (trm_fix f x t).
+..
+
+
+
+--------
+
+
+
+
+
+
+Definition wpgen_fail : formula := mkflocal (fun Q =>
+  \[False]).
+
+Definition wpgen_val (v:val) : formula := mkflocal (fun Q =>
+  Q v).
+
+Definition wpaux_var (E:ctx) (x:var) : formula :=
+  match Ctx.lookup x E with
+  | None => wpgen_fail
+  | Some v => wpgen_val v
+  end.
+
+Definition wpgen_let (F1:formula) (F2of:val->formula) : formula := mkflocal (fun Q =>
+  F1 (fun X => F2of X Q)).
+
+Definition wpgen_seq (F1 F2:formula) : formula := mkflocal (fun Q =>
+  F1 (fun X => F2 Q)).
+
+Definition wpgen_app (t1:trm) (t2:trm) : formula := mkflocal (fun Q =>  
+  wp (trm_app t1 t2) Q)
+
+Definition wpgen_if_val (v:val) (F1 F2:formula) : formula := mkflocal (fun Q =>
+  \exists (b:bool), \[v = val_bool b] \* (if b then F1 Q else F2 Q)).
+
+Definition wpgen_if (F0 F1 F2:formula) : formula :=
+  wpgen_let F0 (fun v => wpgen_if_val v F1 F2).
+
+Fixpoint wpgen (E:ctx) (t:trm) : formula :=
+  let aux := wpgen E in
+  match t with
+  | trm_val v => wpgen_val v
+  | trm_var x => wpaux_var E x
+  | trm_fun x t1 => trm_fun (isubst (Ctx.rem x E) t1)
+  | trm_fix f x t1 => trm_fix (isubst (Ctx.rem x (Ctx.rem f E)) t1))
+  | trm_if t0 t1 t2 => wpgen_if (aux t0) (aux t1) (aux t2)
+  | trm_let x t1 t2 => wpgen_let (aux t1) (fun X => wpgen (Ctx.add x X E) t2)
+  | trm_app t1 t2 => wgpen_app (isubst E t1) (isubst E t2)
+  end.
+
+
+
+
+
+
+
 forward proof 
 - with let
 - lets
