theories/SLFWand.v
@@ -35,6 +35,143 @@ Notation "'\Top''" := hgc.
 (** ** The magic wand *)
 
 (* ------------------------------------------------------- *)
+(** *** A subtraction operator *)
+
+(** At a high level, [H1 \* H2] describes the "addition" of a
+    heap satisfying [H1] with a heap satisfying [H2]. 
+    Think of it as [H1 + H2].
+
+    As a counterpart to this addition operator, we introduce
+    a subtraction operator, written [H1 \-* H2]. 
+    Think of it as [ -H1 + H2].
+
+    A heap [h] satisfies [H1 \-* H2] if and only if, when we augment
+    it with a disjoint heap [h'] satisfying [H1], we recover [H2].
+    Think of it as [(-H1 + H2) + H1] simplifying to [H2].
+
+    The definition of [hwand] follows. *)
+
+Definition hwand (H1 H2:hprop) : hprop :=
+  fun h => forall h', fmap_disjoint h h' -> H1 h' -> H2 (h \u h').
+
+Notation "H1 \-* H2" := (hwand H1 H2) (at level 43).
+
+(** The definition of [hwand] is not easy to make sense of at first.
+    To better grasp its meaning, we next present two alternative
+    definitions of [hwand], and detail its introduction and elimination
+    lemmas. *)
+
+(** The operator [H1 \-* H2] is uniquely defined by the followig
+    equivalence. In other words, any operator that satisfies this
+    equivalence for all arguments is provably equal to the definition 
+    of [hwand] given above. (We proof this fact further in the chapter.) *)
+
+Parameter hwand_characterization : forall H0 H1 H2,
+  (H0 ==> H1 \-* H2) <-> (H0 \* H1 ==> H2).
+
+(** The right-to-left direction is an introduction rule: it tells
+    what needs to be proved to introduce a magic wand [H1 \-* H2]
+    when starting from a state described by [H0]. What needs to
+    be proved is that [H0], if augmented with [H1], yields [H2]. *)
+
+Lemma hwand_intro : forall H0 H1 H2,
+  (H0 \* H1) ==> H2 ->
+  H0 ==> (H1 \-* H2).
+Proof using. intros. applys hwand_characterization. Qed.
+
+(** The left-to-right direction is an elimination rule: it tells
+    what can be deduced from [H0 ==> (H1 \-* H2)]. What can be
+    deduced is that if [H0] is augmented with [H1], then [H2]
+    can be recovered. *)
+
+Lemma hwand_elim : forall H1 H2 H3,
+  H0 ==> (H1 \-* H2) ->
+  (H0 \* H1) ==> H2.
+Proof using. intros. applys hwand_characterization. Qed.
+
+(** This elimination rule can be equivalently reformulated in the
+    following form, which makes it perhaps even clearer that 
+    [H1 \-* H2], when augmented with [H1], yields [H2]. 
+    Think of it as [H1 + (-H1 + H2)] simplifying to [H2]. *)
+
+Lemma hwand_elim' : forall H1 H2,
+  H1 \* (H1 \-* H2) ==> H2.
+Proof using. intros. applys hwand_elim. Qed.
+
+(** Another possible definition of [H1 \-* H2] can be stated
+    without refering to heaps at all, by reusing the basic
+    Separation Logic operators that we have already introduced. 
+    [H1 \-* H2] denotes some heap, described as [H0], such 
+    that [H0] augmented with [H1] yields [H2]. 
+    
+    In the alternative definition of [hwand] shown below,
+    the heap [H0] is existentially quantified using [\exists], 
+    and the entailment assertion is described as the pure heap
+    predicate [\[ H0 \* H1 ==> H2 ]]. *)
+
+Definition hwand' (H1 H2:hprop) : hprop :=
+  \exists H0, H0 \* \[ (H0 \* H1) ==> H2].
+
+(** In practice, [SepBase] relies on the definition of [hwand'],
+    which has the benefit that all properties of [hwand] can be
+    established with help of the tactic [hsimpl]. In other words,
+    we reduce the amount of work by conducting all the reasoning
+    at the level of [hprop] and avoiding the need to work with
+    explicit heaps (of type [heap]). *)
+
+
+(* ------------------------------------------------------- *)
+(** *** Equivalence between the definitions of magic wand *)
+
+(** In what follows we prove the equivalence between the three
+    characterizations of [hwand H1 H2] that we have presented:
+
+    1. [fun h => forall h', fmap_disjoint h h' -> H1 h' -> H2 (h \u h')]
+
+    2. [\exists H0, H0 \* \[ (H0 \* H1) ==> H2]]
+
+    3. [forall H0 H1 H2, (H0 ==> hwand H1 H2) <-> (H0 \* H1 ==> H2)].
+
+    To prove the 3-way equivalence, we first prove the equivalence
+    between (1) and (2), then prove the equivalence between (2) and (3).
+*)
+
+(** Prove that [hwand] is equivalent to [hwand']. *)
+
+Lemma hwand_eq_hwand' :
+  hwand = hwand'.
+Proof using. Qed.
+
+
+(** Prove that [hwand'] satisfies the lemma 
+    [hwand_characterization]. *)
+
+Lemma hwand'_satisfies_hwand_characterization : forall H0 H1 H2,
+  (H0 ==> hwand' H1 H2) <-> (H0 \* H1 ==> H2).
+Proof using. Qed.
+
+Lemma hwand'_satisfies_hwand_characterization' : forall op,
+  op = hwand ->
+  (forall H0 H1 H2, (H0 ==> op H1 H2) <-> (H0 \* H1 ==> H2)).
+Proof using. intros. subst. applys hwand'_satisfies_hwand_characterization. Qed.
+
+(** Reciprocally, show that any operator satisfying
+    [hwand] characterization is equal to [hwand']. *)
+
+Lemma hwand_characterization_eq_hwand' : forall op,
+  (forall H0 H1 H2, (H0 ==> op H1 H2) <-> (H0 \* H1 ==> H2)) ->
+  op = hwand'.
+Proof using. Qed.
+
+
+
+
+
+
+
+
+
+(* ------------------------------------------------------- *)
 (** *** Intuitive interpretation for [hwand] *)
 
 (** In first approximation, [H1 \-* H2] is like [H2] but with 
@@ -60,6 +197,36 @@ Parameter hwand_elim : forall H1 H2,
 
 Parameter hwand_trans_elim : forall H1 H2 H3,
   (H1 \-* H2) \* (H2 \-* H3) ==> (H1 \-* H3).
+
+(** Intuitively, it is safe to replace a heap predicate by another
+    one, if the inequalities required to justified that the first
+    heap predicate makes sense (i.e. that is does not contain 
+    "negative values") are sufficient to justify that the second
+    heap predicate also makes sense.
+    
+    For example, in [(H1 \-* H2) \* (H2 \-* H3) ==> (H1 \-* H3)]
+    the LHS requires [H1 <= H2] and [H2 <= H3], from which we can
+    deduce [H1 <= H3], as required to justify to RHS. 
+  
+    But the reciprocal entailment does not hold: from [H1 <= H3], 
+    we could not possibly justify [H1 <= H2] not [H2 <= H3].
+
+    Likewise, we can prove:
+*)
+
+Lemma hempty_himpl_hwand_self : forall H,
+  \[] ==> (H \-* H).
+Proof using. hsimpl. Qed.
+
+(* FALSE! 
+Lemma hwand_self_himpl_hempty : forall H,
+  (H \-* H) ==> \[].
+Proof using.
+  intros. intros h M. rewrite hwand_eq_hexists_hstar_hpure in M.
+  lets (H'&R): hexists_inv M.
+Qed.
+*)
+
 
 (** Because we are working with heap predicates, and that "negative"
     heap predicates don't quite make sense, we have to be careful.
@@ -92,34 +259,78 @@ Proof using.
   applys hempty_intro. rewrite hstar_hpure in K. destruct K. auto.
 Qed.
 
-(** Intuitively, it is safe to replace a heap predicate by another
-    one, if the inequalities required to justified that the first
-    heap predicate makes sense (i.e. that is does not contain 
-    "negative values") are sufficient to justify that the second
-    heap predicate also makes sense.
-    
-    For example, in [(H1 \-* H2) \* (H2 \-* H3) ==> (H1 \-* H3)]
-    the LHS requires [H1 <= H2] and [H2 <= H3], from which we can
-    deduce [H1 <= H3], as required to justify to RHS. 
-  
-    But the reciprocal entailment does not hold: from [H1 <= H3], 
-    we could not possibly justify [H1 <= H2] not [H2 <= H3].
 
-    Likewise, we can prove:
-*)
+(* ------------------------------------------------------- *)
 
-Lemma hempty_himpl_hwand_self : forall H,
-  \[] ==> (H \-* H).
-Proof using. hsimpl. Qed.
+intro rule
 
-(* FALSE! 
-Lemma hwand_self_himpl_hempty : forall H,
-  (H \-* H) ==> \[].
-Proof using.
-  intros. intros h M. rewrite hwand_eq_hexists_hstar_hpure in M.
-  lets (H'&R): hexists_inv M.
-Qed.
-*)
+  H1 \* H2 ==> H3 ->
+  H1 ==> H2 \-* H3
+
+elim rule
+
+   H1 ==> H2 \-* H3 ->
+   H1 \* H2 ==> H3
+
+equivalence of elim rule
+
+  H1 \* (H1 \-* H2) ==> H2.
+
+
+
+-----------------------------
+
+not that reciprocal is false!
+
+  H2 ==> H1 \* (H1 \-* H2) 
+
+
+
+
+(* ------------------------------------------------------- *)
+(** *** Frame expressed with [hwand]: the ramified frame rule *)
+
+
+
+
+
+
+  H ==> H1 \* H2 ->
+  triple t H1 Q1 ->
+  Q1 \* H2 ==> Q \*+ \GC ->
+  triple t H Q
+
+
+  H ==> H1 \* H2 ->
+  triple t H1 Q1 ->
+  Q1 \* H2 ==> Q \*+ \GC ->
+  triple t H Q
+
+
+
+  H ==> H1 \* H2 ->
+  triple t H1 Q1 ->
+  H2 ==> Q1 \*- (Q \*+ \GC) ->
+  triple t H Q
+
+
+  H ==> H1 \* (Q1 \*- (Q \*+ \GC)) ->
+  triple t H1 Q1 ->
+  triple t H Q
+
+reciprocally frame derivable
+
+  H ==> H1 \* H2 ->
+  triple t H1 Q1 ->
+  H2 ==> Q1 \*- (Q \*+ \GC) ->
+  triple t H Q
+
+
+  MQ. H ==> H1 \* (Q1 \*- (Q \*+ \GC))
+  MQ. H1 \* H2  ==> H1 \* (Q1 \*- (Q \*+ \GC))
+  MQ. H2  ==> (Q1 \*- (Q \*+ \GC))
+  MQ. Q1 \* H2  ==> (Q \*+ \GC)
+  done.
 
 
 
@@ -134,3 +345,95 @@ Qed.
     when augmenting [h] with a heap [h'] that satisfies [H1],
 
 *)
+
+
+Lemma flocal_elim : forall F H Q,
+  H ==> wp t Q' \* (Q' \--* (Q \*+ \GC)) ->
+  H ==> wp t Q.
+Proof using. introv L M. lets N: (L Q). applys* himpl_trans N. Qed.
+
+
+
+
+
+  prove1: 
+    F Q ==> mklocal F Q
+    (take Q1 = Q)
+
+  prove 2:
+    (mkflocal (mkflocal F)) Q := mkflocal F
+    right-to-left : instance of (1)
+    left-to-right: ...
+
+    (mkflocal (mkflocal F)) Q
+  = \exists Q1, mkflocal F Q1 \* (Q1 \--* (Q \*+ \GC))
+  = \exists Q1, (\exists Q2, F Q2 \* (Q2 \--* (Q1 \*+ \GC))) \* (Q1 \--* (Q \*+ \GC))
+  = \exists Q1 Q2, F Q2 \* (Q2 \--* (Q1 \*+ \GC) \* (Q1 \--* (Q \*+ \GC))
+  = \exists Q1 Q2, F Q2 \* (Q2 \--* (Q1 \*+ \GC) \* ((Q1 \*+ \GC) \--* ((Q \*+ \GC) \*+ \GC))
+  ==> \exists Q1 Q2, F Q2 \* (Q2 \--* (Q1 \*+ \GC) \* ((Q1 \*+ \GC) \--* (Q \*+ \GC \*+ \GC))
+  = \exists Q1 Q2, F Q2 \* (Q2 \--* (Q \*+ \GC \*+ \GC))
+  = \exists Q2, F Q2 \* (Q2 \--* (Q \*+ \GC))
+  = mkflocal F
+
+
+  mkflocal F Q := \exists Q1, F Q1 \* (Q1 \--* (Q \*+ \GC)).
+
+  \exists Q1, F Q1 \* (Q1 \--* (Q \*+ \GC)) ==> F Q
+
+
+  F Q1 \* (Q1 \--* (Q \*+ \GC)) ==> F Q
+
+
+
+  wp t Q1 \* (Q1 \--* (Q \*+ \GC)) ==> wp t Q
+
+
+  H ==> wp t Q1 \* (Q1 \--* (Q \*+ \GC)) ->
+  H ==> wp t Q.
+
+
+let H1 := wp t Q1
+let H2 := (Q1 \--* (Q \*+ \GC)) 
+
+
+  H ==> H1 \* H2 ->
+  H1 ==> wp t Q1 ->
+  Q1 \* H2 ==> Q \*+ \GC ->
+  H ==> wp t Q.
+
+
+  H ==> H1 \* H2 ->
+  triple t H1 Q1 ->
+  Q1 \* H2 ==> Q \*+ \GC ->
+  triple t H Q
+
+
+reciprocally, with 
+   forall Q1,   wp t Q1 \* (Q1 \--* (Q \*+ \GC)) ==> wp t Q
+we can simulate frame
+
+
+  H ==> H1 \* H2 ->
+  H1 ==> wp t Q1 ->
+  Q1 \* H2 ==> Q \*+ \GC ->
+  H ==> wp t Q.
+
+exploit fact
+
+  H ==> H1 \* H2 ->
+  H1 ==> wp t Q1 ->
+  Q1 \* H2 ==> Q \*+ \GC ->
+  H ==> wp t Q1 \* (Q1 \--* (Q \*+ \GC))
+
+suffices (hchange 1 and 2)
+
+  H1 \* H2 ==> wp t Q1 \* (Q1 \--* (Q \*+ \GC))
+  wp t Q1 \* H2 ==> wp t Q1 \* (Q1 \--* (Q \*+ \GC))
+  H2 ==> (Q1 \--* (Q \*+ \GC))
+
+done.
+
+
+
+
+
